finished alpha equivalence definitions for comparing states' alpha equivalence

Transformations/Renamer_DeBruijn_Ext_Correct.thy
@@ -3,28 +3,197 @@ theory Renamer_DeBruijn_Ext_Correct
 
 begin
 
-(* alpha equivalence modulo a set of scopes *)
+type_synonym subst =
+  "(YulIdentifier * YulIdentifier) list list"
+
+definition subst_get1 :: "subst \<Rightarrow> YulIdentifier list list" where
+"subst_get1 s =
+  map (map fst) s"
+
+definition subst_get2 :: "subst \<Rightarrow> YulIdentifier list list" where
+"subst_get2 s =
+  map (map snd) s"
+
+definition subst_flip :: "subst \<Rightarrow> subst" where
+"subst_flip s =
+  map (map (\<lambda> p . case p of (x, y) \<Rightarrow> (y, x))) s"
+
+(* alpha equivalence modulo a set of scopes 
+ * s1 and s2 probably need different scopes here *)
 definition alpha_equiv_statement' ::
-  "YulIdentifier list list \<Rightarrow> ('v, 't) YulStatement \<Rightarrow> ('v, 't) YulStatement \<Rightarrow> bool" where
+  "subst \<Rightarrow> ('v, 't) YulStatement \<Rightarrow> ('v, 't) YulStatement \<Rightarrow> bool" where
 "alpha_equiv_statement' scopes s1 s2 =
-  (yul_statement_to_deBruijn scopes s1 = yul_statement_to_deBruijn scopes s2)"
+  (yul_statement_to_deBruijn (subst_get1 scopes) s1 =
+   yul_statement_to_deBruijn (subst_get2 scopes) s2)"
 
 definition alpha_equiv_expr' ::
-  "YulIdentifier list list \<Rightarrow> ('v, 't) YulExpression \<Rightarrow> ('v, 't) YulExpression \<Rightarrow> bool" where
+  "subst \<Rightarrow> ('v, 't) YulExpression \<Rightarrow> ('v, 't) YulExpression \<Rightarrow> bool" where
 "alpha_equiv_expr' scopes s1 s2 =
-  (yul_expr_to_deBruijn scopes s1 = yul_expr_to_deBruijn scopes s2)"
+  (yul_expr_to_deBruijn (subst_get1 scopes) s1 =
+  yul_expr_to_deBruijn (subst_get2 scopes) s2)"
 
 (*
  * 
  *)
+
+definition alpha_equiv_statement ::
+  "('v, 't) YulStatement \<Rightarrow> ('v, 't) YulStatement \<Rightarrow> bool" where
+"alpha_equiv_statement s1 s2 =
+  alpha_equiv_statement' [] s1 s2"
+
+definition alpha_equiv_expr ::
+  "('v, 't) YulExpression \<Rightarrow> ('v, 't) YulExpression \<Rightarrow> bool" where
+"alpha_equiv_expr s1 s2 =
+  alpha_equiv_expr' [] s1 s2"
+
+fun subst1 :: "subst \<Rightarrow> YulIdentifier \<Rightarrow> YulIdentifier option" where
+"subst1 [] _ = None"
+| "subst1 (h#t) v =
+   (case map_of h v of
+    None \<Rightarrow> subst1 t v
+    | Some v' \<Rightarrow> Some v')"
+
+fun subst_list :: "subst \<Rightarrow> YulIdentifier list \<Rightarrow> YulIdentifier list option" where
+"subst_list _ [] = Some []"
+| "subst_list s (vh#vt) =
+   (case subst1 s vh of
+    None \<Rightarrow> None
+    | Some vh' \<Rightarrow>
+      (case subst_list s vt of
+       None \<Rightarrow> None
+       | Some vt' \<Rightarrow> Some (vh'#vt')))"
+
+(* for function bodies that are builtins, we need to be able to
+ * rename parameters. might want to find a way to share code for doing this
+ *)
+
+fun rename_locals :: "subst \<Rightarrow> 'v locals \<Rightarrow> 'v locals option" where
+"rename_locals _ [] = Some []"
+| "rename_locals s ((n, v)#t) =
+   (case subst1 s n of
+    None \<Rightarrow> None
+    | Some n' \<Rightarrow>
+    (case rename_locals s t of
+      None \<Rightarrow> None
+      | Some t' \<Rightarrow> (Some ((n', v)#t'))))"
+
+(* NB: this may be too strong a notion for other uses, as it
+ * depends on the ordering of values in the locals. However for
+ * our purposes it should be fine since the states will be exactly the same
+ * even in terms of structure, apart from names.
+ *)
+fun alpha_equiv_locals' ::
+  "subst \<Rightarrow> 'v locals \<Rightarrow> 'v locals \<Rightarrow> bool" where
+"alpha_equiv_locals' subst [] [] = True"
+| "alpha_equiv_locals' subst ((n1, v1)#t1) ((n2, v2)#t2) =
+   (subst1 subst n1 = Some n2 \<and>
+    v1 = v2 \<and>
+    alpha_equiv_locals' subst t1 t2)"
+| "alpha_equiv_locals' _ _ _ = False"
+
+definition alpha_equiv_function_sig'_scheme ::
+  "subst \<Rightarrow> YulIdentifier \<Rightarrow> ('g, 'v, 't, 'z) function_sig'_scheme \<Rightarrow> YulIdentifier \<Rightarrow> ('g, 'v, 't, 'z) function_sig'_scheme \<Rightarrow> bool" where
+"alpha_equiv_function_sig'_scheme subst n1 s1 n2 s2 =
+  (subst1 subst n1 = Some n2 \<and>
+  (case (f_sig_body s1, f_sig_body s2) of
+        (YulBuiltin b1, YulBuiltin b2) \<Rightarrow>
+          (let args1 = (map (\<lambda> x . case x of (YulTypedName n t) \<Rightarrow> n) (f_sig_arguments s1)) in
+          (let args2 = (map (\<lambda> x . case x of (YulTypedName n t) \<Rightarrow> n) (f_sig_arguments s2)) in
+          (let rets1 = (map (\<lambda> x . case x of (YulTypedName n t) \<Rightarrow> n) (f_sig_returns s1)) in
+          (let rets2 = (map (\<lambda> x . case x of (YulTypedName n t) \<Rightarrow> n) (f_sig_returns s2)) in
+            ((subst_list subst args1 = Some args2) \<and> (subst_list subst rets1 = Some rets2))))))
+        | (YulFunction sts1, YulFunction sts2) \<Rightarrow>
+            alpha_equiv_statement' subst 
+              (YulFunctionDefinitionStatement (YulFunctionDefinition n1 (f_sig_arguments s1) (f_sig_returns s1) sts1))
+              (YulFunctionDefinitionStatement (YulFunctionDefinition n2 (f_sig_arguments s2) (f_sig_returns s2) sts2))
+        | (_, _) \<Rightarrow> False))"
+
+(* alpha_equiv_function_sig - compare visible ids *)
+definition alpha_equiv_function_sig' ::
+  "subst \<Rightarrow> YulIdentifier \<Rightarrow> ('g, 'v, 't) function_sig \<Rightarrow> YulIdentifier \<Rightarrow> ('g, 'v, 't) function_sig \<Rightarrow> bool" where
+"alpha_equiv_function_sig' subst n1 s1 n2 s2 =
+  (subst_list subst (f_sig_visible s1) = Some (f_sig_visible s2) \<and>
+   alpha_equiv_function_sig'_scheme subst n1 s1 n2 s2)"
+
+(*
+fun alpha_equiv_function_bodies' ::
+  "subst \<Rightarrow> ('g, 'v, 't) YulFunctionBody \<Rightarrow> ('g, 'v, 't) YulFunctionBody \<Rightarrow> bool" where
+"alpha_equiv_function_bodies subst (YulBuiltin f1) (YulBuiltin f2) = (f1 = f2)"
+| "alpha_equiv_function_bodies subst (YulFunction sts1) (YulFunction sts2) =
+    alpha_equiv_statement' subst
+      (YulFunctionDefinitionStatement (YulFunctionDefinition n1 (f_sig_arguments s1) (f_sig_returns s1) (f_sig_body s1)))
+      (YulFunctionDefinitionStatement (YulFunctionDefinition n2 (f_sig_arguments s2) (f_sig_returns s2) (f_sig_body s2)))"
+*)
+
+(* TODO: we aren't checking that types are compatible here. Perhaps this can be done
+ * in a different pass *)
+fun alpha_equiv_funs' ::
+  "subst \<Rightarrow> ('g, 'v, 't) function_sig locals \<Rightarrow> ('g, 'v, 't) function_sig locals \<Rightarrow> bool"
+  where
+"alpha_equiv_funs' subst [] [] = True"
+| "alpha_equiv_funs' subst ((n1, s1)#t1) ((n2, s2)#t2) =
+   (alpha_equiv_function_sig' subst n1 s1 n2 s2 \<and>
+    alpha_equiv_funs' subst t1 t2)"
+| "alpha_equiv_funs' _ _ _ = False"
+
+(* YOU ARE HERE *)
+(* TODO: make sure we are handling equivalence of function-contexts correctly.
+ * this is a bit complicated to due to possibility of recursion/mutual recursion *)
+
+fun alpha_equiv_stackEl' ::
+  "subst \<Rightarrow> ('g, 'v, 't) StackEl \<Rightarrow> ('g, 'v, 't) StackEl \<Rightarrow> bool" where
+"alpha_equiv_stackEl' subst (EnterStatement s1) (EnterStatement s2) =
+  alpha_equiv_statement' subst s1 s2"
+| "alpha_equiv_stackEl' subst (ExitStatement s1 vs1 fs1) (ExitStatement s2 vs2 fs2) =
+    (alpha_equiv_statement' subst s1 s2 \<and>
+     alpha_equiv_locals' subst vs1 vs2 \<and>
+     alpha_equiv_funs' subst fs1 fs2)"
+| "alpha_equiv_stackEl' subst (Expression e1) (Expression e2) =
+  alpha_equiv_expr' subst e1 e2"
+| "alpha_equiv_stackEl' subst (EnterFunctionCall n1 f1) (EnterFunctionCall n2 f2) = 
+   (alpha_equiv_function_sig' subst n1 f1 n2 f2)"
+| "alpha_equiv_stackEl' subst (ExitFunctionCall n1 vals1 locals1 fs1 f1)
+                              (ExitFunctionCall n2 vals2 locals2 fs2 f2) =
+    (alpha_equiv_function_sig' subst n1 f1 n2 f2 \<and>
+     alpha_equiv_locals' subst locals1 locals2 \<and>
+     alpha_equiv_funs' subst fs1 fs2)"
+| "alpha_equiv_stackEl' subst _ _ = False"
+
+
+(* YulSemanticsSingleStep.result *)
+
+definition alpha_equiv_results' ::
+  "subst \<Rightarrow>
+   ('g, 'v, 't) YulSemanticsSingleStep.result \<Rightarrow>
+   ('g, 'v, 't) YulSemanticsSingleStep.result \<Rightarrow>
+   bool" where
+"alpha_equiv_results' subst r1 r2 =
+  (global r1 = global r2 \<and>
+   vals r1 = vals r2 \<and>
+   alpha_equiv_locals' subst (locals r1) (locals r2) \<and>
+   alpha_equiv_locals' subst (funs r1) (funs r2) \<and>
+   (list_all2 (alpha_equiv_stackEl' subst)
+              (cont r1)
+              (cont r2)))"
 
 (* Idea: if both programs take a step, then
  * the results are the same (up to alpha equivalence of states)
  * This also means we need to be able to account for alpha-equivalent input
  * states, in order to make this work.
  *)
+
 (*
-lemma alpha_equiv_correct_full :
-  
+ * TODO: will scopes change during the execution of
+ * a step?
+ *)
+(*
+lemma alpha_equiv_correct_step_noerr :
+  assumes H: "alpha_equiv_results' scopes s1 s2"
+  assumes H1: "evalYulStep d s1 = Result s1'"
+  shows "\<exists> s2' . evalYulStep d s2 = Result s2' \<and>
+           alpha_equiv_results' scopes s1' s2'"
+
+proof
+
 *)
 end
